src/cursorprops.v
@@ -22,3 +22,4 @@ Proof.
   rewrite addB1.
   congruence.
 Qed.
+
